# 7. Fibers

This is a literate `rzk` file:

```rzk
#lang rzk-1
```

## Fibers

The homotopy fiber of a map is the following type:

```rzk title="The fiber of a map"
#def fib
  ( A B : U)
  ( f : A → B)
  ( b : B)
  : U
  := Σ (a : A) , (f a) = b
```

We calculate the transport of `#!rzk (a , q) : fib b` along `#!rzk p : a = a'`:

```rzk
#def transport-in-fiber
  ( A B : U)
  ( f : A → B)
  ( b : B)
  ( a a' : A)
  ( u : (f a) = b)
  ( p : a = a')
  : ( transport A ( \ x → (f x) = b) a a' p u) =
    ( concat B (f a') (f a) b (ap A B a' a f (rev A a a' p)) u)
  :=
    ind-path
      ( A)
      ( a)
      ( \ a'' p' →
        ( transport (A) (\ x → (f x) = b) (a) (a'') (p') (u)) =
        ( concat (B) (f a'') (f a) (b) (ap A B a'' a f (rev A a a'' p')) (u)))
      ( rev
        ( (f a) = b) (concat B (f a) (f a) b refl u) (u)
        ( left-unit-concat B (f a) b u))
      ( a')
      ( p)
```

### Induction principle for fibers

The family of fibers has the following induction principle: To prove/construct
something about/for every point in every fiber, it suffices to do so for points
of the form `#!rzk (a, refl : f a = f a) : fib A B f`.

```rzk
#def ind-fib
  ( A B : U)
  ( f : A → B)
  ( C : (b : B) → fib A B f b → U)
  ( s : (a : A) → C (f a) (a, refl))
  ( b : B)
  ( (a, q) : fib A B f b)
  : C b (a, q)
  :=
    ind-path B (f a) (\ b p → C b (a, p)) (s a) b q

#def ind-fib-computation
  ( A B : U)
  ( f : A → B)
  ( C : (b : B) → fib A B f b → U)
  ( s : (a : A) → C (f a) (a, refl))
  ( a : A)
  : ind-fib A B f C s (f a) (a, refl) = s a
  := refl
```

### Functoriality of fibers

```rzk
#def map-of-fibers-map-of-maps
  ( A' A : U)
  ( α : A' → A)
  ( B' B : U)
  ( β : B' → B)
  ( ((s', s), square-commutes) : map-of-maps A' A α B' B β)
  ( a : A)
  : fib A' A α a → fib B' B β (s a)
  :=
  ( ind-fib A' A α)
  ( \ x _ → fib B' B β (s x))
  ( \ x' →  (s' x', square-commutes x'))
  ( a)

#def compute-map-of-fibers-map-of-maps
  ( A' A : U)
  ( α : A' → A)
  ( B' B : U)
  ( β : B' → B)
  ( ((s', s), square-commutes) : map-of-maps A' A α B' B β)
  ( a : A)
  ( (a', p) : fib A' A α a)
  : ( ( map-of-fibers-map-of-maps A' A α B' B β)
      ( (s', s), square-commutes)
      ( a)
      ( a', p)
    = ( s' a'
      , ( concat B (β (s' a')) (s (α a')) (s a))
        ( square-commutes a')
        ( ap A B (α a') a s p)))
  :=
  ( ind-fib A' A α)
  ( \ x (x', h) →
    ( ( map-of-fibers-map-of-maps A' A α B' B β)
      ( (s', s), square-commutes)
      ( x)
      ( x', h)
    = ( s' x'
      , ( concat B (β (s' x')) (s (α x')) (s x))
        ( square-commutes x')
        ( ap A B (α x') x s h))))
  ( \ x' → refl )
  ( a)
  ( a', p)
```

Note that due to how `#!rzk ind-fib` is implemented,
`#!rzk map-of-fibers-map-of-maps {-snip-} (α a') a' (a', refl)` is
_definitionally_ equal to `#!rzk (s' a', square-commutes a')`, so we don't need
`#!rzk compute-map-of-fibers-map-of-maps` in that case.

```rzk
#def homotopy-identity-of-fiber-identity-of-map
  ( A' A : U)
  ( α : A' → A)
  ( a : A)
  ( u : fib A' A α a)
  : map-of-fibers-map-of-maps A' A α A' A α (identity-of-map A' A α) a u = u
  :=
  ( ind-fib A' A α)
  ( \ x z →
    map-of-fibers-map-of-maps A' A α A' A α (identity-of-map A' A α) x z = z)
  ( ind-fib-computation A' A α (\ x _ → fib A' A α x) (\ x' →  (x', refl)))
  ( a)
  ( u)

#def homotopy-comp-maps-of-fibers-comp-maps-of-maps
  ( A' A : U)
  ( α : A' → A)
  ( B' B : U)
  ( β : B' → B)
  ( C' C : U)
  ( γ : C' → C)
  ( ((t', t), second-square-commutes) : map-of-maps B' B β C' C γ)
  ( ((s', s), first-square-commutes) : map-of-maps A' A α B' B β)
  ( a : A)
  ( u : fib A' A α a)
  : ( ( map-of-fibers-map-of-maps B' B β C' C γ)
      ( (t', t), second-square-commutes)
      ( s a)
      ( ( map-of-fibers-map-of-maps A' A α B' B β)
        ( (s', s), first-square-commutes)
        ( a)
        ( u))
    = ( ( map-of-fibers-map-of-maps A' A α C' C γ)
        ( ( comp-maps-of-maps A' A α B' B β C' C γ)
          ( (t', t), second-square-commutes)
          ( (s', s), first-square-commutes))
        ( a)
        ( u)))
  :=
  ( ind-fib A' A α)
  ( \ x z →
    ( ( map-of-fibers-map-of-maps B' B β C' C γ)
      ( (t', t), second-square-commutes)
      ( s x)
      ( ( map-of-fibers-map-of-maps A' A α B' B β)
        ( (s', s), first-square-commutes)
        ( x)
        ( z))
    = ( ( map-of-fibers-map-of-maps A' A α C' C γ)
        ( ( comp-maps-of-maps A' A α B' B β C' C γ)
          ( (t', t), second-square-commutes)
          ( (s', s), first-square-commutes))
        ( x)
        ( z))))
  ( \ x' →
    -- Here we only need one application of `compute-map-of-fibers-of-maps`
    -- because of the definitional computation rule for
    -- `map-of-fibers-map-of-maps {-snip-} (x', refl)` mentioned above.
    ( ( compute-map-of-fibers-map-of-maps B' B β C' C γ)
      ( (t', t), second-square-commutes)
      ( s (α x'))
      ( s' x', first-square-commutes x')))
  ( a)
  ( u)
```

## Contractible maps

A map is contractible just when its fibers are contractible.

```rzk title="Contractible maps"
#def is-contr-map
  ( A B : U)
  ( f : A → B)
  : U
  := (b : B) → is-contr (fib A B f b)
```

### Contractible maps are equivalences

Contractible maps are equivalences:

```rzk
#section is-equiv-is-contr-map

#variables A B : U
#variable f : A → B
#variable is-contr-f : is-contr-map A B f
```

```rzk title="The inverse to a contractible map"
#def is-contr-map-inverse
  : B → A
  := \ b → first (center-contraction (fib A B f b) (is-contr-f b))

#def has-section-is-contr-map
  : has-section A B f
  :=
    ( is-contr-map-inverse ,
      \ b → second (center-contraction (fib A B f b) (is-contr-f b)))

#def is-contr-map-data-in-fiber uses (is-contr-f)
  (a : A)
  : fib A B f (f a)
  := (is-contr-map-inverse (f a) , (second has-section-is-contr-map) (f a))

#def is-contr-map-path-in-fiber
  (a : A)
  : (is-contr-map-data-in-fiber a) =_{fib A B f (f a)} (a , refl)
  :=
    all-elements-equal-is-contr
      ( fib A B f (f a))
      ( is-contr-f (f a))
      ( is-contr-map-data-in-fiber a)
      ( a , refl)

#def is-contr-map-has-retraction uses (is-contr-f)
  : has-retraction A B f
  :=
    ( is-contr-map-inverse ,
      \ a → ( ap (fib A B f (f a)) A
                ( is-contr-map-data-in-fiber a)
                ( (a , refl))
                ( \ u → first u)
                ( is-contr-map-path-in-fiber a)))

#def is-equiv-is-contr-map uses (is-contr-f)
  : is-equiv A B f
  := (is-contr-map-has-retraction , has-section-is-contr-map)

#end is-equiv-is-contr-map
```

### Half adjoint equivalences are contractible maps

We prove the converse by fiber induction. To define the contracting homotopy to
the point `#!rzk (f a, refl)` in the fiber over `#!rzk f a` we find it easier to
work from the assumption that `f` is a half adjoint equivalence.

```rzk
#section is-contr-map-is-equiv

#variables A B : U
#variable f : A → B
#variable is-hae-f : is-half-adjoint-equiv A B f

#def is-split-surjection-is-half-adjoint-equiv
  ( b : B)
  : fib A B f b
  :=
    ( map-inverse-is-half-adjoint-equiv A B f is-hae-f b,
      section-htpy-is-half-adjoint-equiv A B f is-hae-f b)

#def calculate-is-split-surjection-is-half-adjoint-equiv
  ( a : A)
  : is-split-surjection-is-half-adjoint-equiv (f a) = (a, refl)
  :=
    path-of-pairs-pair-of-paths
    ( A)
    ( \ a' → f a' = f a)
    ( map-inverse-is-half-adjoint-equiv A B f is-hae-f (f a))
    ( a)
    ( retraction-htpy-is-half-adjoint-equiv A B f is-hae-f a)
    ( section-htpy-is-half-adjoint-equiv A B f is-hae-f (f a))
    ( refl)
    ( triple-concat
      ( f a = f a)
      ( transport A ( \ x → (f x) = (f a))
        ( map-inverse-is-half-adjoint-equiv A B f is-hae-f (f a))
        ( a)
        ( retraction-htpy-is-half-adjoint-equiv A B f is-hae-f a)
        ( section-htpy-is-half-adjoint-equiv A B f is-hae-f (f a)))
      ( concat B
        ( f a)
        ( f (map-inverse-is-half-adjoint-equiv A B f is-hae-f (f a)))
        ( f a)
        ( ap A B
          ( a)
          ( map-inverse-is-half-adjoint-equiv A B f is-hae-f (f a))
          ( f)
          ( rev A ( map-inverse-is-half-adjoint-equiv A B f is-hae-f (f a)) a
            ( retraction-htpy-is-half-adjoint-equiv A B f is-hae-f a)))
        ( section-htpy-is-half-adjoint-equiv A B f is-hae-f (f a)))
      ( concat B
        ( f a)
        ( f (map-inverse-is-half-adjoint-equiv A B f is-hae-f (f a)))
        ( f a)
        ( ap A B
          ( a)
          ( map-inverse-is-half-adjoint-equiv A B f is-hae-f (f a))
          ( f)
          ( rev A (map-inverse-is-half-adjoint-equiv A B f is-hae-f (f a)) a
            ( retraction-htpy-is-half-adjoint-equiv A B f is-hae-f a)))
        ( ap A B (map-inverse-is-half-adjoint-equiv A B f is-hae-f (f a)) a f
          ( retraction-htpy-is-half-adjoint-equiv A B f is-hae-f a)))
      ( refl)
      ( transport-in-fiber A B f (f a)
        ( map-inverse-is-half-adjoint-equiv A B f is-hae-f (f a))
        ( a)
        ( section-htpy-is-half-adjoint-equiv A B f is-hae-f (f a))
        ( retraction-htpy-is-half-adjoint-equiv A B f is-hae-f a))
      ( concat-eq-right B
        ( f a)
        ( f (map-inverse-is-half-adjoint-equiv A B f is-hae-f (f a)))
        ( f a)
        ( ap A B
          ( a)
          ( map-inverse-is-half-adjoint-equiv A B f is-hae-f (f a))
          ( f)
          ( rev A ( map-inverse-is-half-adjoint-equiv A B f is-hae-f (f a)) a
            ( retraction-htpy-is-half-adjoint-equiv A B f is-hae-f a)))
        ( section-htpy-is-half-adjoint-equiv A B f is-hae-f (f a))
        ( ap A B (map-inverse-is-half-adjoint-equiv A B f is-hae-f (f a)) a f
          ( retraction-htpy-is-half-adjoint-equiv A B f is-hae-f a))
        (coherence-is-half-adjoint-equiv A B f is-hae-f a))
      ( concat-ap-rev-ap-id A B
        ( map-inverse-is-half-adjoint-equiv A B f is-hae-f (f a))
        ( a)
        ( f)
        ( retraction-htpy-is-half-adjoint-equiv A B f is-hae-f a)))

#def contraction-fib-is-half-adjoint-equiv uses (is-hae-f)
  ( b : B)
  ( z : fib A B f b)
  : is-split-surjection-is-half-adjoint-equiv b = z
  :=
    ind-fib
    ( A) (B) (f)
    ( \ b' z' → is-split-surjection-is-half-adjoint-equiv b' = z')
    ( calculate-is-split-surjection-is-half-adjoint-equiv)
    ( b)
    ( z)

#def is-contr-map-is-half-adjoint-equiv uses (is-hae-f)
  : is-contr-map A B f
  :=
    \ b →
      ( is-split-surjection-is-half-adjoint-equiv b,
        contraction-fib-is-half-adjoint-equiv b)

#end is-contr-map-is-equiv
```

### Equivalences are contractible maps

```rzk
#def is-contr-map-is-equiv
  ( A B : U)
  ( f : A → B)
  ( is-equiv-f : is-equiv A B f)
  : is-contr-map A B f
  :=
    \ b →
    ( is-split-surjection-is-half-adjoint-equiv A B f
      ( is-half-adjoint-equiv-is-equiv A B f is-equiv-f) b ,
      \ z → contraction-fib-is-half-adjoint-equiv A B f
        ( is-half-adjoint-equiv-is-equiv A B f is-equiv-f) b z)

#def is-contr-map-iff-is-equiv
  ( A B : U)
  ( f : A → B)
  : iff (is-contr-map A B f) (is-equiv A B f)
  := (is-equiv-is-contr-map A B f , is-contr-map-is-equiv A B f)
```

## Fibers of projections

For a family of types `#!rzk B : A → U`, the fiber of the projection from
`#!rzk total-type A B` to `#!rzk A` over `#!rzk a : A` is equivalent to
`#!rzk B a`. While both types deserve the name "fibers" to disambiguate, we
temporarily refer to the fiber as the "homotopy fiber" and `#!rzk B a` as the
"strict fiber."

```rzk
#section strict-vs-homotopy-fiber

#variable A : U
#variable B : A → U

#def homotopy-fiber-strict-fiber
  (a : A)
  (b : B a)
  : fib (total-type A B) A (projection-total-type A B) a
  := ((a, b), refl)

#def strict-fiber-homotopy-fiber
  (a : A)
  (((a', b'), p) : fib (total-type A B) A (projection-total-type A B) a)
  : B a
  := transport A B a' a p b'

#def retract-homotopy-fiber-strict-fiber
  (a : A)
  (b : B a)
  : strict-fiber-homotopy-fiber a (homotopy-fiber-strict-fiber a b) = b
  := refl

#def calculation-retract-strict-fiber-homotopy-fiber
  (a : A)
  (b : B a)
  : homotopy-fiber-strict-fiber a
    ( strict-fiber-homotopy-fiber a ((a, b), refl)) =
    ( (a, b), refl)
  := refl

#def retract-strict-fiber-homotopy-fiber
  (a : A)
  (((a', b'), p) : fib (total-type A B) A (projection-total-type A B) a)
  : homotopy-fiber-strict-fiber a (strict-fiber-homotopy-fiber a ((a', b'), p))
    = ((a', b'), p)
  :=
    ind-fib
    ( total-type A B)
    ( A)
    ( projection-total-type A B)
    ( \ a0 ((a'', b''), p') →
      homotopy-fiber-strict-fiber a0
      ( strict-fiber-homotopy-fiber a0 ((a'', b''), p')) = ((a'', b''), p'))
    ( \ (a'', b'') → refl)
    ( a)
    ( ((a', b'), p))

#def equiv-homotopy-fiber-strict-fiber
  (a : A)
  : Equiv
    ( B a)
    ( fib (total-type A B) A (projection-total-type A B) a)
  :=
    ( homotopy-fiber-strict-fiber a,
      ( ( strict-fiber-homotopy-fiber a,
          retract-homotopy-fiber-strict-fiber a),
        ( strict-fiber-homotopy-fiber a,
          retract-strict-fiber-homotopy-fiber a)))

#end strict-vs-homotopy-fiber
```

## Fibers of composites

The fiber of a composite function is a sum over the fiber of the second function
of the fibers of the first function.

```rzk
#section fiber-composition

#variables A B C : U
#variable f : A → B
#variable g : B → C

#def fiber-sum-fiber-comp
  (c : C)
  ((a, r) : fib A C (comp A B C g f) c)
  : ( Σ ((b, q) : fib B C g c), fib A B f b)
  := ((f a, r), (a, refl))

#def fiber-comp-fiber-sum
  (c : C)
  ( ((b, q), (a, p)) : Σ ((b, q) : fib B C g c), fib A B f b)
  : fib A C (comp A B C g f) c
  := (a, concat C (g (f a)) (g b) c (ap B C (f a) b g p) q)

#def is-retract-fiber-sum-fiber-comp
  (c : C)
  ((a, r) : fib A C (comp A B C g f) c)
  : fiber-comp-fiber-sum c (fiber-sum-fiber-comp c (a, r)) = (a, r)
  :=
    eq-eq-fiber-Σ
    ( A)
    ( \ a0 → (g (f a0)) = c)
    ( a)
    ( concat C (g (f a)) (g (f a)) c refl r)
    ( r)
    ( left-unit-concat C (g (f a)) c r)

#def is-retract-fiber-comp-fiber-sum'
  (c : C)
  ((b, q) : fib B C g c)
  : ((a, p) : fib A B f b) →
    fiber-sum-fiber-comp c (fiber-comp-fiber-sum c ((b, q), (a, p))) =
    ((b, q), (a, p))
  :=
    ind-fib B C g
    ( \ c' (b', q') → ((a, p) : fib A B f b') →
      fiber-sum-fiber-comp c' (fiber-comp-fiber-sum c' ((b', q'), (a, p))) =
      ((b', q'), (a, p)))
    ( \ b0 (a, p) →
      ( ind-fib A B f
        ( \b0' (a', p') →
          fiber-sum-fiber-comp (g b0')
          ( fiber-comp-fiber-sum (g b0') ((b0', refl), (a', p'))) =
          ((b0', refl), (a', p')))
        ( \a0 → refl)
        ( b0)
        ( (a, p))))
    ( c)
    ( (b, q))

#def is-retract-fiber-comp-fiber-sum
  (c : C)
  ( ((b, q), (a, p)) : Σ ((b, q) : fib B C g c), fib A B f b)
  : fiber-sum-fiber-comp c (fiber-comp-fiber-sum c ((b, q), (a, p))) =
    ((b, q), (a, p))
  := is-retract-fiber-comp-fiber-sum' c (b, q) (a, p)

#def equiv-fiber-sum-fiber-comp
  (c : C)
  : Equiv
    ( fib A C (comp A B C g f) c)
    ( Σ ((b, q) : fib B C g c), fib A B f b)
  :=
    ( fiber-sum-fiber-comp c,
      ( ( fiber-comp-fiber-sum c,
          is-retract-fiber-sum-fiber-comp c),
        ( fiber-comp-fiber-sum c,
          is-retract-fiber-comp-fiber-sum c)))

#end fiber-composition
```
